theories/proofmode/monpred.v
@@ -486,12 +486,18 @@ Global Instance add_modal_at_fupd_goal `{BiFUpd PROP} E1 E2 𝓟 𝓟' Q i :
   AddModal 𝓟 𝓟' (|={E1,E2}=> Q i) → AddModal 𝓟 𝓟' ((|={E1,E2}=> Q) i).
 Proof. by rewrite /AddModal !monPred_at_fupd. Qed.
 
-Global Instance elim_inv_embed φ 𝓟inv 𝓟in 𝓟out Pin Pout Q Q' :
-  (∀ i, ElimInv φ 𝓟inv 𝓟in 𝓟out (Q i) (Q' i)) →
+Global Instance elim_inv_embed φ 𝓟inv 𝓟in 𝓟out 𝓟close Pin Pout Pclose Q Q' :
+  (∀ i, ElimInv φ 𝓟inv 𝓟in 𝓟out 𝓟close (Q i) (Q' i)) →
   MakeEmbed 𝓟in Pin → MakeEmbed 𝓟out Pout →
-  ElimInv φ ⎡𝓟inv⎤ Pin Pout Q Q'.
+  match 𝓟close, Pclose with
+  | Some 𝓟close, Some Pclose => MakeEmbed 𝓟close Pclose
+  | None, None => True
+  | _, _ => False
+  end →
+  ElimInv φ ⎡𝓟inv⎤ Pin Pout Pclose Q Q'.
 Proof.
-  rewrite /MakeEmbed /ElimInv=>H <- <- ?. iStartProof PROP.
-  iIntros (?) "(?&?&HQ')". iApply H; [done|]. iFrame. iIntros "?". by iApply "HQ'".
+  rewrite /MakeEmbed /ElimInv=>H <- <- Hclose ?. iStartProof PROP.
+  iIntros (?) "(?&?&HQ')". iApply H; [done|]. iFrame. iIntros "?".
+  destruct 𝓟close; destruct Pclose; try rewrite -Hclose; iApply "HQ'"; done.
 Qed.
 End sbi.
