theories/tests/proofmode_iris.v
@@ -67,6 +67,14 @@ Section iris_tests.
     iModIntro. iSplit; auto.
   Qed.
 
+  Lemma test_iInv_0_with_close N P: inv N (<pers> P) ={⊤}=∗ ▷ P.
+  Proof.
+    iIntros "#H".
+    iInv N as "#H2" "Hclose".
+    iMod ("Hclose" with "H2").
+    iModIntro. by iNext.
+  Qed.
+
   Lemma test_iInv_1 N E P:
     ↑N ⊆ E →
     inv N (<pers> P) ={E}=∗ ▷ P.
@@ -82,6 +90,15 @@ Section iris_tests.
     iIntros "(#?&?)".
     iInv N as "(#HP&Hown)".
     iModIntro. iSplit; auto with iFrame.
+  Qed.
+
+  Lemma test_iInv_2_with_close γ p N P:
+    cinv N γ (<pers> P) ∗ cinv_own γ p ={⊤}=∗ cinv_own γ p ∗ ▷ P.
+  Proof.
+    iIntros "(#?&?)".
+    iInv N as "(#HP&Hown)" "Hclose".
+    iMod ("Hclose" with "HP").
+    iModIntro. iFrame. by iNext.
   Qed.
 
   Lemma test_iInv_3 γ p1 p2 N P:
@@ -101,6 +118,18 @@ Section iris_tests.
     iIntros (?) "(#?&Hown1&Hown2)".
     iInv N as "(#HP&Hown2)".
     iModIntro. iSplitL "Hown2"; auto with iFrame.
+  Qed.
+
+  Lemma test_iInv_4_with_close t N E1 E2 P:
+    ↑N ⊆ E2 →
+    na_inv t N (<pers> P) ∗ na_own t E1 ∗ na_own t E2
+         ⊢ |={⊤}=> na_own t E1 ∗ na_own t E2  ∗ ▷ P.
+  Proof.
+    iIntros (?) "(#?&Hown1&Hown2)".
+    iInv N as "(#HP&Hown2)" "Hclose".
+    iMod ("Hclose" with "[HP Hown2]").
+    { iFrame. done. }
+    iModIntro. iFrame. by iNext.
   Qed.
 
   (* test named selection of which na_own to use *)
